The Formula for the Fibonacci sequence is as follows </br>
![F_{n}=F_{n-1}-F_{n-2}](https://render.githubusercontent.com/render/math?math=F_%7Bn%7D%3DF_%7Bn-1%7D-F_%7Bn-2%7D) </br>
typically ![F_{0}=0 , F_{1} = 1 , F_{2}=1 , F_{3}=2](https://render.githubusercontent.com/render/math?math=F_%7B0%7D%3D0%20%2C%20F_%7B1%7D%20%3D%201%20%2C%20F_%7B2%7D%3D1%20%2C%20F_%7B3%7D%3D2) </br>
Since each term the Fibonacci sequence is the sum of the two previous ones, a term would only be even when the two previous are both odd. By extending the the Fibonacci sequence back to 0. the first even number is at N=3, with the next ones being at N=6, N=9 and so on. Therefor a Fibonacci number N is even if N mod 3 = 0. 
